Hoare/While/DenotationalSemantics.lean
@@ -1,5 +1,6 @@
 import Hoare.While.Syntax
 import Hoare.While.Context
+import Hoare.While.Types
 
 namespace While
 
@@ -81,5 +82,182 @@ instance decideVal? {Γ : Context} {e : Expr} : Decidable (e.val? Γ =  some (Va
     X := X + 1
   od
 〛
+
+def Val.ty : Val → Ty
+  | num _ => .num
+  | bool _ => .bool
+
+def Expr.val_ty (e : Expr) (t : Ty) : Prop :=
+  ∀ Γ, ∀ val, (e.val? Γ = .some val) → val.ty = t
+
+theorem Expr.val_add {e₁ e₂ : Expr} {val : Val} {Γ : Context} :
+   (Expr.add e₁ e₂).val? Γ = val →
+  ∃ n₁ n₂, e₁.val? Γ = Val.num n₁ ∧ e₂.val? Γ = Val.num n₂ ∧ val = Val.num (n₁ + n₂) := by
+  intro h
+  simp [val?] at h
+  split at h
+  · case h_1 x1 x2 n1 n2 heq1 heq2 =>
+      exists n1; exists n2
+      exact ⟨heq1, ⟨heq2, Option.some_inj.1 h |>.symm⟩⟩
+  · case h_2 x1 x2 hx =>
+      contradiction
+
+theorem Expr.val_sub {e₁ e₂ : Expr} {val : Val} {Γ : Context} :
+   (Expr.sub e₁ e₂).val? Γ = val →
+  ∃ n₁ n₂, e₁.val? Γ = Val.num n₁ ∧ e₂.val? Γ = Val.num n₂ ∧ val = Val.num (n₁ - n₂) := by
+  intro h
+  simp [val?] at h
+  split at h
+  · case h_1 x1 x2 n1 n2 heq1 heq2 =>
+      exists n1; exists n2
+      exact ⟨heq1, ⟨heq2, Option.some_inj.1 h |>.symm⟩⟩
+  · case h_2 x1 x2 hx =>
+      contradiction
+
+theorem Expr.val_mul {e₁ e₂ : Expr} {val : Val} {Γ : Context} :
+   (Expr.mul e₁ e₂).val? Γ = val →
+  ∃ n₁ n₂, e₁.val? Γ = Val.num n₁ ∧ e₂.val? Γ = Val.num n₂ ∧ val = Val.num (n₁ * n₂) := by
+  intro h
+  simp [val?] at h
+  split at h
+  · case h_1 x1 x2 n1 n2 heq1 heq2 =>
+      exists n1; exists n2
+      exact ⟨heq1, ⟨heq2, Option.some_inj.1 h |>.symm⟩⟩
+  · case h_2 x1 x2 hx =>
+      contradiction
+
+theorem Expr.val_eq {e₁ e₂ : Expr} {val : Val} {Γ : Context} :
+   (Expr.eq e₁ e₂).val? Γ = val →
+  (∃ n₁ n₂, e₁.val? Γ = Val.num n₁ ∧ e₂.val? Γ = Val.num n₂ ∧ val = Val.bool (n₁ == n₂)) ∨
+  (∃ b₁ b₂, e₁.val? Γ = Val.bool b₁ ∧ e₂.val? Γ = Val.bool b₂ ∧ val = Val.bool (b₁ == b₂)) := by
+  intro h
+  simp [val?] at h
+  split at h
+  · case h_1 x1 x2 n1 n2 heq1 heq2 =>
+      left; exists n1; exists n2
+      exact ⟨heq1, ⟨heq2, Option.some_inj.1 h |>.symm⟩⟩
+  · case h_2 x1 x2 b1 b2 heq1 heq2 =>
+      right; exists b1; exists b2
+      exact ⟨heq1, ⟨heq2, Option.some_inj.1 h |>.symm⟩⟩
+  · case h_3 x1 x2 hx =>
+      contradiction
+
+theorem Expr.val_lt {e₁ e₂ : Expr} {val : Val} {Γ : Context} :
+   (Expr.lt e₁ e₂).val? Γ = val →
+  ∃ n₁ n₂, e₁.val? Γ = Val.num n₁ ∧ e₂.val? Γ = Val.num n₂ ∧ val = Val.bool (n₁ < n₂) := by
+  intro h
+  simp [val?] at h
+  split at h
+  · case h_1 x1 x2 n1 n2 heq1 heq2 =>
+      exists n1; exists n2
+      exact ⟨heq1, ⟨heq2, Option.some_inj.1 h |>.symm⟩⟩
+  · case h_2 x1 x2 hx =>
+      contradiction
+
+theorem Expr.val_gt {e₁ e₂ : Expr} {val : Val} {Γ : Context} :
+   (Expr.gt e₁ e₂).val? Γ = val →
+  ∃ n₁ n₂, e₁.val? Γ = Val.num n₁ ∧ e₂.val? Γ = Val.num n₂ ∧ val = Val.bool (n₁ > n₂) := by
+  intro h
+  simp [val?] at h
+  split at h
+  · case h_1 x1 x2 n1 n2 heq1 heq2 =>
+      exists n1; exists n2
+      exact ⟨heq1, ⟨heq2, Option.some_inj.1 h |>.symm⟩⟩
+  · case h_2 x1 x2 hx =>
+      contradiction
+
+theorem Expr.val_le {e₁ e₂ : Expr} {val : Val} {Γ : Context} :
+   (Expr.lt e₁ e₂).val? Γ = val →
+  ∃ n₁ n₂, e₁.val? Γ = Val.num n₁ ∧ e₂.val? Γ = Val.num n₂ ∧ val = Val.bool (n₁ ≤ n₂) := by
+  intro h
+  simp [val?] at h
+  split at h
+  · case h_1 x1 x2 n1 n2 heq1 heq2 =>
+      exists n1; exists n2
+      exact ⟨heq1, ⟨heq2, Option.some_inj.1 h |>.symm⟩⟩
+  · case h_2 x1 x2 hx =>
+      contradiction
+
+theorem Expr.val_gt {e₁ e₂ : Expr} {val : Val} {Γ : Context} :
+   (Expr.gt e₁ e₂).val? Γ = val →
+  ∃ n₁ n₂, e₁.val? Γ = Val.num n₁ ∧ e₂.val? Γ = Val.num n₂ ∧ val = Val.bool (n₁ > n₂) := by
+  intro h
+  simp [val?] at h
+  split at h
+  · case h_1 x1 x2 n1 n2 heq1 heq2 =>
+      exists n1; exists n2
+      exact ⟨heq1, ⟨heq2, Option.some_inj.1 h |>.symm⟩⟩
+  · case h_2 x1 x2 hx =>
+      contradiction
+
+| le : Expr → Expr → Expr
+| ge : Expr → Expr → Expr
+| and : Expr → Expr → Expr
+| or : Expr → Expr → Expr
+
+theorem Expr.well_typed_val {t : Ty} {e : Expr} : WellTyped e t ↔ e.val_ty t := by
+  constructor
+  · case mp =>
+      intro h Γ val hval
+      have hval := hval.symm
+      have ht := WellTyped.ty_some h
+      induction e generalizing val
+      · case num => simp [Expr.ty] at ht; simp [val?] at hval; subst ht; subst hval; simp [Val.ty]
+      · case bool => simp [Expr.ty] at ht; simp [val?] at hval; subst ht; subst hval; simp [Val.ty]
+      · case var => simp [Expr.ty] at ht
+      · case add e₁ e₂ ihe₁ ihe₂ ihv =>
+          cases h
+          case add ihwt₁ ihwt₂ =>
+            simp [val?] at ihv
+            have ⟨n1, n2, ⟨hn₁, hn₂, hnval⟩⟩ := Expr.val_add hval.symm
+            rw [hnval]
+            simp [Val.ty]
+      · case sub e₁ e₂ ihe₁ ihe₂ ihv =>
+          cases h
+          case sub ihwt₁ ihwt₂ =>
+            simp [val?] at ihv
+            have ⟨n1, n2, ⟨hn₁, hn₂, hnval⟩⟩ := Expr.val_sub hval.symm
+            rw [hnval]
+            simp [Val.ty]
+      · case mul e₁ e₂ ihe₁ ihe₂ ihv =>
+          cases h
+          case mul ihwt₁ ihwt₂ =>
+            simp [val?] at ihv
+            have ⟨n1, n2, ⟨hn₁, hn₂, hnval⟩⟩ := Expr.val_mul hval.symm
+            rw [hnval]
+            simp [Val.ty]
+      · case eq e₁ e₂ ihe₁ ihe₂ ihv =>
+          cases h
+          case eq ihwt₁ ihwt₂ =>
+            simp [val?] at ihv
+            cases Expr.val_eq hval.symm
+            · case inl hexists =>
+              have ⟨n1, n2, ⟨hn₁, hn₂, hnval⟩⟩ := hexists
+              rw [hnval]
+              simp [Val.ty]
+            · case inr hexists =>
+              have ⟨n1, n2, ⟨hn₁, hn₂, hnval⟩⟩ := hexists
+              rw [hnval]
+              simp [Val.ty]
+      · case lt e₁ e₂ ihe₁ ihe₂ ihv =>
+
+
+
+
+
+
+
+
+
+
+
+
+
+
+
+
+
+
+
 
 end While
